examples/dsls/mini_steel/tests/Pulse.Tests.fst
@@ -1,123 +1,148 @@
 module Pulse.Tests
 module T = FStar.Tactics
-open Pulse.Steel.Wrapper
 open Pulse.Syntax
 open Pulse.Main
 open Steel.ST.Util 
 open Steel.ST.Reference
+open Pulse.Steel.Wrapper
 open Steel.FractionalPermission
 open FStar.Ghost
 #push-options "--print_universes --print_implicits"
+let expects = ()
+let provides = ()
 
-%splice_t[foo] (parse_and_check "return true")
 
-%splice_t[read] (parse_and_check "
-   fun (n:FStar.Ghost.erased u#0 Pulse.Steel.Wrapper.u32)
-       (r:Steel.ST.Reference.ref Pulse.Steel.Wrapper.u32)
-         requires (Steel.ST.Reference.pts_to #Pulse.Steel.Wrapper.u32 r Steel.FractionalPermission.full_perm (FStar.Ghost.reveal u#0 #Pulse.Steel.Wrapper.u32 n)) ->
-         Pulse.Steel.Wrapper.read n r
-   ")
+(* Start up the solver and feed it the initial context *)
+let warmup (x:int) = assert (x + 1 > x)
 
-%splice_t[read2] (check (`(fun (n:erased u#0 u32) (r:ref u32) ->
-                              Pulse.Steel.Wrapper.read n r 
-                            <: stt u#0 u32
-                                (pts_to #u32 r full_perm (reveal u#0 #u32 n))
-                                (fun x -> pts_to #u32 r full_perm x))))
+%splice_t[test_true] (check (`(true)))
 
-%splice_t[read_alt_with_post] (parse_and_check "
-    fun (n:FStar.Ghost.erased u#0 Pulse.Steel.Wrapper.u32)
-        (r:Steel.ST.Reference.ref Pulse.Steel.Wrapper.u32)   
-          requires  (Steel.ST.Reference.pts_to #Pulse.Steel.Wrapper.u32 r Steel.FractionalPermission.full_perm (FStar.Ghost.reveal u#0 #Pulse.Steel.Wrapper.u32 n))
-          ensures _ . (Steel.ST.Reference.pts_to #Pulse.Steel.Wrapper.u32 r Steel.FractionalPermission.full_perm 
-                                                (FStar.Ghost.reveal u#0 #Pulse.Steel.Wrapper.u32 n)) ->
-          Pulse.Steel.Wrapper.read_alt n r
-    ")
+%splice_t[test_syntax] (check  (`(
+   fun (x:ref u32) (#n:erased u#0 u32) -> 
+     (expects (
+        pts_to x full_perm (reveal n)))
+     (provides (fun _ ->
+        pts_to x full_perm 0ul))
+     (
+       let _ = write n x 1ul in
+       write (hide u#0 #u32 1ul) x 0ul
+     )
+   )))
 
- %splice_t[read_alt_with_post2] (parse_and_check "
-   fun (n:FStar.Ghost.erased u#0 Pulse.Steel.Wrapper.u32)
-       (r1:Steel.ST.Reference.ref Pulse.Steel.Wrapper.u32)
-       (r2:Steel.ST.Reference.ref Pulse.Steel.Wrapper.u32)
-         requires  (Steel.ST.Reference.pts_to #Pulse.Steel.Wrapper.u32 r1 Steel.FractionalPermission.full_perm (FStar.Ghost.reveal u#0 #Pulse.Steel.Wrapper.u32 n) *
-                    Steel.ST.Reference.pts_to #Pulse.Steel.Wrapper.u32 r2 Steel.FractionalPermission.full_perm (FStar.Ghost.reveal u#0 #Pulse.Steel.Wrapper.u32 n))
-         ensures _ . (Steel.ST.Reference.pts_to #Pulse.Steel.Wrapper.u32 r1 Steel.FractionalPermission.full_perm (FStar.Ghost.reveal u#0 #Pulse.Steel.Wrapper.u32 n) *
-                      Steel.ST.Reference.pts_to #Pulse.Steel.Wrapper.u32 r2 Steel.FractionalPermission.full_perm (FStar.Ghost.reveal u#0 #Pulse.Steel.Wrapper.u32 n)) ->
-         Pulse.Steel.Wrapper.read_alt n r2
-   ")
+%splice_t[test_read2] (check (`(
+  fun (n:erased u#0 u32) (r:ref u32) ->
+    (expects (
+       pts_to r full_perm (reveal n)))
+    (provides (fun x ->
+       pts_to r full_perm x))
+    (
+       read n r 
+    )
+)))       
 
-%splice_t[read_refine] (parse_and_check "
-    fun (n:FStar.Ghost.erased u#0 Pulse.Steel.Wrapper.u32)
-        (r:Steel.ST.Reference.ref Pulse.Steel.Wrapper.u32)
-           requires (Steel.ST.Reference.pts_to #Pulse.Steel.Wrapper.u32 r Steel.FractionalPermission.full_perm (FStar.Ghost.reveal u#0 #Pulse.Steel.Wrapper.u32 n)) ->
-           Pulse.Steel.Wrapper.read_refine n r
-     ")
+%splice_t[test_read_alt_with_post] (check (`(
+  fun (n:erased u#0 u32)
+    (r:ref u32) ->
+    (expects (
+       pts_to r full_perm (reveal n)))
+    (provides (fun _ -> 
+       pts_to r full_perm (reveal n)))
+    (
+       read_alt n r
+    )
+)))
 
- %splice_t[write] (parse_and_check "
-    fun (n:FStar.Ghost.erased u#0 Pulse.Steel.Wrapper.u32)
-        (r1:Steel.ST.Reference.ref Pulse.Steel.Wrapper.u32)
-        (x:Pulse.Steel.Wrapper.u32)
-        (r2:Steel.ST.Reference.ref Pulse.Steel.Wrapper.u32)
-          requires (Steel.ST.Reference.pts_to #Pulse.Steel.Wrapper.u32 r1 Steel.FractionalPermission.full_perm (FStar.Ghost.reveal u#0 #Pulse.Steel.Wrapper.u32 n) *
-                    Steel.ST.Reference.pts_to #Pulse.Steel.Wrapper.u32 r2 Steel.FractionalPermission.full_perm (FStar.Ghost.reveal u#0 #Pulse.Steel.Wrapper.u32 n)) ->
-          Pulse.Steel.Wrapper.write n r2 x
-    ")
+%splice_t[test_read_alt_with_post2] (check (`(
+    fun (n:erased u#0 u32)
+      (r1 r2:ref u32) ->
+      (expects (
+         pts_to r1 full_perm (reveal n) `star`
+         pts_to r2 full_perm (reveal n)))
+      (provides (fun _ -> 
+         pts_to r1 full_perm (reveal n) `star`
+         pts_to r2 full_perm (reveal n)))
+      (
+         read_alt n r2
+      )
+)))
+
+%splice_t[test_read_refine] (check (`(
+      fun (n:erased u#0 u32)
+        (r:ref u32) ->
+        (expects (
+           pts_to r full_perm (reveal n)))
+        (
+           read_refine n r
+        )
+)))
+
+%splice_t[test_write] (check (`(
+     fun (n:erased u#0 u32)
+       (r1:ref u32)
+       (x:u32)
+       (r2:ref u32) ->
+       (expects (
+          pts_to r1 full_perm (reveal n) `star`
+          pts_to r2 full_perm (reveal n)))
+       (
+          write n r2 x
+       )
+)))
 
 //Bound variable escapes scope
 [@@ expect_failure]
- %splice_t[read_alt_write] (parse_and_check  "
-     fun (n:FStar.Ghost.erased u#0 Pulse.Steel.Wrapper.u32)
-         (r:Steel.ST.Reference.ref Pulse.Steel.Wrapper.u32)
-           requires (Steel.ST.Reference.pts_to #Pulse.Steel.Wrapper.u32 r Steel.FractionalPermission.full_perm 
-                                               (FStar.Ghost.reveal u#0 #Pulse.Steel.Wrapper.u32 n)) ->
-           let x = Pulse.Steel.Wrapper.read_alt n r;
-           Pulse.Steel.Wrapper.write n r x
-     ")
+%splice_t[test_read_alt_write] (check (`(
+  fun (n:erased u#0 u32)
+    (r:ref u32) ->
+    (expects (
+       pts_to r full_perm (reveal n)))
+    (
+       let x = read_alt n r in
+       write n r x
+    )
+)))
 
-
-%splice_t[read_alt_write_alt] (parse_and_check  "
-      fun (n:FStar.Ghost.erased u#0 Pulse.Steel.Wrapper.u32)
-          (r:Steel.ST.Reference.ref Pulse.Steel.Wrapper.u32)
-           requires (Steel.ST.Reference.pts_to #Pulse.Steel.Wrapper.u32 r Steel.FractionalPermission.full_perm 
-                                               (FStar.Ghost.reveal u#0 #Pulse.Steel.Wrapper.u32 n)) ->
-            let x = Pulse.Steel.Wrapper.read_alt n r;
-            Pulse.Steel.Wrapper.write_alt n r x
-      ")
-
-%splice_t[swap] (parse_and_check "
-    fun (n1:FStar.Ghost.erased u#0 Pulse.Steel.Wrapper.u32)
-        (n2:FStar.Ghost.erased u#0 Pulse.Steel.Wrapper.u32)
-        (r1:Steel.ST.Reference.ref Pulse.Steel.Wrapper.u32)
-        (r2:Steel.ST.Reference.ref Pulse.Steel.Wrapper.u32)
-          requires (Steel.ST.Reference.pts_to #Pulse.Steel.Wrapper.u32 r1 Steel.FractionalPermission.full_perm (FStar.Ghost.reveal u#0 #Pulse.Steel.Wrapper.u32 n1) *
-                    Steel.ST.Reference.pts_to #Pulse.Steel.Wrapper.u32 r2 Steel.FractionalPermission.full_perm (FStar.Ghost.reveal u#0 #Pulse.Steel.Wrapper.u32 n2))
-          ensures _.(Steel.ST.Reference.pts_to #Pulse.Steel.Wrapper.u32 r1 Steel.FractionalPermission.full_perm (FStar.Ghost.reveal u#0 #Pulse.Steel.Wrapper.u32 n2) *
-                     Steel.ST.Reference.pts_to #Pulse.Steel.Wrapper.u32 r2 Steel.FractionalPermission.full_perm (FStar.Ghost.reveal u#0 #Pulse.Steel.Wrapper.u32 n1)) ->
-          let x = Pulse.Steel.Wrapper.read_refine n1 r1;
-          let y = Pulse.Steel.Wrapper.read_refine n2 r2;
-          Pulse.Steel.Wrapper.write n1 r1 y;
-          Pulse.Steel.Wrapper.write n2 r2 x
-    ")
 
 [@@ expect_failure]
-%splice_t[read_implicit] (parse_and_check "
-  fun (#n:FStar.Ghost.erased u#0 Pulse.Steel.Wrapper.u32)
-      (r:Steel.ST.Reference.ref Pulse.Steel.Wrapper.u32)
-        requires (Steel.ST.Reference.pts_to #Pulse.Steel.Wrapper.u32 r Steel.FractionalPermission.full_perm (FStar.Ghost.reveal u#0 #Pulse.Steel.Wrapper.u32 n)) ->
-        Pulse.Steel.Wrapper.read_implicit r
-  ")
+%splice_t[read_implicit] (check (`(
+  fun (#n:erased u#0 u32)
+    (r:ref u32) ->
+    (expects (
+       pts_to r full_perm (reveal n)))
+    (
+       read_implicit r
+    )
+)))
+    
+%splice_t[test_swap2] (check (`(
+  fun (n1 n2:erased u#0 u32)
+    (r1 r2:ref u32) ->
+    (expects  (
+      pts_to r1 full_perm (reveal n1) `star` 
+      pts_to r2 full_perm (reveal n2)))
+    (provides (fun _ ->
+      pts_to r1 full_perm (reveal n2) `star` 
+      pts_to r2 full_perm (reveal n1)))
+    (
+      let x = read_refine n1 r1 in
+      let y = read_refine n2 r2 in
+      write n1 r1 y;
+      write n2 r2 x
+    )
+)))
 
-//This one doesn't work yet ... some bug in translating the quoted term
-[@@expect_failure]
-%splice_t[swap2] (check (`(fun (n1 n2:erased u#0 u32)
-                             (r1 r2:ref u32) ->
-                        (let x = read_refine n1 r1 in
-                         let y = read_refine n2 r2 in
-                         write n1 r1 y;
-                         write n2 r2 x) <:
-                         stt u#0 unit 
-                          (pts_to #u32 r1 full_perm (reveal u#0 #u32 n1) `star` 
-                           pts_to #u32 r2 full_perm (reveal u#0 #u32 n2))
-                          (fun _ -> 
-                           pts_to #u32 r1 full_perm (reveal u#0 #u32 n2) `star` 
-                           pts_to #u32 r2 full_perm (reveal u#0 #u32 n1)))))
 
-
+%splice_t[call_swap2] (check (`(
+  fun (n1 n2:erased u#0 u32)
+    (r1 r2:ref u32) ->
+    (expects  (
+      pts_to r1 full_perm (reveal n1) `star` 
+      pts_to r2 full_perm (reveal n2)))
+    (provides (fun _ -> 
+      pts_to r1 full_perm (reveal n1) `star` 
+      pts_to r2 full_perm (reveal n2)))
+    (
+      test_swap2 n1 n2 r1 r2;
+      test_swap2 n2 n1 r1 r2
+    )
+)))
